Cleanup groupoid

groupoid.v
@@ -11,56 +11,236 @@ Set Default Goal Selector "!".
 
 Require Import Coq.Unicode.Utf8.
 Require Import Coq.Strings.String.
+Require Import Coq.Program.Wf.
+Require Import Coq.Arith.PeanoNat.
+Require Import FunInd.
+
+Import IfNotations.
+
+Reserved Notation "'some' x .. y , P"
+         (at level 200, x binder, y binder, right associativity,
+          format "'[ ' '[ ' 'some'  x .. y ']' ,  '/' P ']'").
+Reserved Notation "'Σ' x .. y , P"
+         (at level 200, x binder, y binder, right associativity,
+          format "'[ ' '[ ' 'Σ'  x .. y ']' ,  '/' P ']'").
+
+#[universes(cumulative)]
+Record someT [A] (P: A → Type) := some_intro { head: A ; tail: P head ; }.
+
+Arguments some_intro [A P].
+Arguments head [A P].
+Arguments tail [A P].
+
+Module Import SomeNotations.
+  Add Printing Let someT.
+
+  Notation "'some' x .. y , P" := (someT (λ x, .. (someT (λ y,  P)) .. )) : type_scope.
+  Notation "'Σ' x .. y , P" := (someT (λ x, .. (someT (λ y,  P)) .. )) : type_scope.
+End SomeNotations.
+
+Inductive U := set | type (n: nat).
+
+Definition U_dec (x y: U): {x = y} + { x ≠ y}.
+Proof.
+  set (s := Nat.eq_dec).
+  decide equality.
+Defined.
+
+Definition succU u :=
+  match u with
+  | set => type 0
+  | type n => type (n + 1)
+  end.
 
 Inductive term :=
-| undef
-| type
-| set
+| ofU (u: U)
+
 | all (x: string) (e0 e1: term)
 
 | var (x: string)
 | lam (x: string) (e0 e1: term)
 | app (e0 e1: term)
 
-| cast (p e0: term)
-| trans (e0 e1: term)
+| compose (e0 e1: term)
 | sym (e: term)
+
 | beta (x: string) (A e0 e1: term)
-| K (e0 e1: term)
 .
-Definition subst x e: term → term :=
-  fix loop (t: term) :=
-    match t with
-    | undef => undef
 
-    | type => type
-    | set => set
-    | all y A e => if string_dec x y then all y (loop A) e else all y (loop A) (loop e)
+Infix "∘" := compose (at level 30).
 
-    | var y => if string_dec x y then e else t
-    | lam y A e => if string_dec x y then lam y (loop A) e else lam y (loop A) (loop e)
-    | app e0 e1 => app (loop e0) (loop e1)
+Coercion ofU: U >-> term.
+Coercion var: string >-> term.
 
-    | cast p e => cast (loop p) (loop e)
-    | trans e0 e1 => trans (loop e0) (loop e1)
-    | sym e => sym (loop e)
-    | K e e' => K (loop e) (loop e')
-    | beta y A f e => if string_dec x y then beta y (loop A) f (loop e) else beta y (loop A) (loop f) (loop e)
-  end.
+Definition term_dec (x y: term): {x = y} + { x ≠ y}.
+Proof.
+  set (u := U_dec).
+  set (s := string_dec).
+  decide equality.
+Defined.
 
-Definition mt (_: string): term := undef.
 Definition put x A (Γ: string → term) : string → term :=
   λ y, if string_dec x y then A else Γ y.
 
+Inductive
+  substs (x: string) (s: term): term → term → Type :=
+| substs_ofU u: substs x s (ofU u) (ofU u)
+
+| substs_var_eq: substs x s (var x) s
+| substs_var_ne y: x ≠ y → substs x s (var y) (var y)
+
+| substs_all_eq A A' e:
+    substs x s A A' →
+    substs x s (all x A e) (all x A' e)
+| substs_all_ne y A A' e e':
+    x ≠ y →
+    substs x s A A' →
+    substs x s e e' →
+    substs x s (all y A e) (all y A' e')
+
+| substs_lam_eq A A' e:
+    substs x s A A' →
+    substs x s (lam x A e) (lam x A' e)
+| substs_lam_ne y A A' e e':
+    x ≠ y →
+    substs x s A A' →
+    substs x s e e' →
+    substs x s (lam y A e) (lam y A' e')
+
+| substs_app e0 e1 e0' e1':
+    substs x s e0 e0' →
+    substs x s e1 e1' →
+    substs x s (app e0 e1) (app e0' e1')
+
+| substs_compose e0 e1 e0' e1':
+    substs x s e0 e0' →
+    substs x s e1 e1' →
+    substs x s (e0 ∘ e1) (e0' ∘ e1')
+| substs_sym e0 e0':
+    substs x s e0 e0' →
+    substs x s (sym e0) (sym e0')
+
+| substs_beta_eq A A' e0 e1 e1':
+    substs x s A A' →
+    substs x s e1 e1' →
+    substs x s (beta x A e0 e1) (beta x A' e0 e1')
+| substs_beta_ne y A A' e0 e0' e1 e1':
+    x ≠ y →
+    substs x s A A' →
+    substs x s e0 e0' →
+    substs x s e1 e1' →
+    substs x s (beta y A e0 e1) (beta y A' e0' e1')
+.
+
+Function subst x s t :=
+  match t with
+  | ofU u => ofU u
+
+  | all y A e => if string_dec x y then all y (subst x s A) e else all y (subst x s A) (subst x s e)
+
+  | var y => if string_dec x y then s else t
+  | lam y A e => if string_dec x y then lam y (subst x s A) e else lam y (subst x s A) (subst x s e)
+  | app e0 e1 => app (subst x s e0) (subst x s e1)
+
+  | e0 ∘ e1 => subst x s e0 ∘ subst x s e1
+  | sym e => sym (subst x s e)
+  | beta y A f e => if string_dec x y then beta y (subst x s A) f (subst x s e) else beta y (subst x s A) (subst x s f) (subst x s e)
+  end.
+Notation "[ x := e0 ]" := (subst x e0).
+
+Definition subst_sound:
+  ∀ {x s e e'},
+  e' = [x := s] e →
+  substs x s e e'.
+Proof.
+  intros x s e.
+  functional induction ([x := s] e).
+  all: intros e' p.
+  all: inversion p.
+  all: subst.
+  all: try econstructor.
+  all: try eauto.
+Defined.
+
+Definition subst_complete:
+  ∀ {x s e e'},
+  substs x s e e' →
+  e' = [x := s] e.
+Proof.
+  intros x s e.
+  induction e.
+  all: intros e' p.
+  all: inversion p.
+  all: subst.
+  all: cbn in *.
+  all: repeat rewrite (IHe1 _ H3).
+  all: repeat rewrite (IHe1 _ H4).
+  all: repeat rewrite (IHe1 _ H5).
+  all: repeat rewrite (IHe3 _ H5).
+  all: repeat rewrite (IHe2 _ H6).
+  all: repeat rewrite (IHe3 _ H7).
+  all: repeat rewrite (IHe _ H0).
+  all: repeat rewrite (IHe1 _ H1).
+  all: repeat rewrite (IHe2 _ H3).
+  all: repeat rewrite (IHe2 _ H5).
+  all: try reflexivity.
+  all: try destruct (string_dec x0 x0).
+  all: try contradiction.
+  all: try reflexivity.
+  all: try destruct (string_dec x x0).
+  all: try contradiction.
+  all: try reflexivity.
+Defined.
+
+
+Reserved Notation "x ; A ≡ B" (at level 80).
+
+Inductive
+  maps: term → term → term → Type :=
+
+| maps_ofU u:
+    ofU u ; ofU u ≡ ofU u
+| maps_var x:
+    var x ; var x ≡ var x
+
+| maps_all x A e p q r s:
+    A ; p ≡ q →
+    e ; r ≡ s →
+    all x A e ; all x p r ≡ all x q s
+
+| maps_lam x A e p q r s:
+    A ; p ≡ q →
+    e ; r ≡ s →
+    lam x A e ; lam x p r ≡ lam x q s
+
+| maps_app e0 e1 p q r s:
+    e0 ; p ≡ q →
+    e1 ; r ≡ s →
+    app e0 e1 ; app p r ≡ app q s
+
+| maps_compose e0 e1 p q r:
+    e0 ; q ≡ r →
+    e1 ; p ≡ q →
+    e0 ∘ e1 ; p ≡ r
+
+| maps_sym e p q:
+    e ; p ≡ q →
+    sym e ; q ≡ p
+
+| maps_beta x A e0 e1 e0':
+    substs x e1 e0 e0' →
+    beta x A e0 e1 ; app (lam x A e0) e1 ≡ e0'
+
+where "x ; A ≡ B" := (maps x A B).
+
 Reserved Notation "Γ ⊢ x ∈ A" (at level 80).
-Reserved Notation "Γ ⊢ x ; A ≡ B" (at level 80).
 
 Inductive
   types (Γ: string → term): term → term → Type :=
 | types_var x: Γ ⊢ var x ∈ Γ x
-| types_set: Γ ⊢ set ∈ type
+| types_ofU u: Γ ⊢ ofU u ∈ ofU (succU u)
 
-| types_all K L x A B:
+| types_all {K L x A B}:
     Γ ⊢ A ∈ K →
     put x A Γ ⊢ B ∈ L →
     Γ ⊢ all x A B ∈ L
@@ -73,63 +253,365 @@ Inductive
 | types_app x e0 e1 A B:
     Γ ⊢ e0 ∈ all x A B →
     Γ ⊢ e1 ∈ A →
-    Γ ⊢ app e0 e1 ∈ subst x e1 B
+    Γ ⊢ app e0 e1 ∈ [x := e1] B
 
-| types_trans A e0 e1:
+| types_compose A B e0 e1:
     Γ ⊢ e0 ∈ A →
-    Γ ⊢ e1 ∈ A →
-    Γ ⊢ trans e0 e1 ∈ A
+    Γ ⊢ e1 ∈ B →
+    Γ ⊢ e0 ∘ e1 ∈ (A ∘ B)
 | types_sym A e:
     Γ ⊢ e ∈ A →
     Γ ⊢ sym e ∈ A
 | types_beta x A B e0 e1:
     Γ ⊢ app (lam x A e0) e1 ∈ B →
-    Γ ⊢ subst x e1 e0 ∈ B →
+    Γ ⊢ [x := e1] e0 ∈ B →
     Γ ⊢ beta x A e0 e1 ∈ B
-| types_K e e' A:
-    Γ ⊢ e ∈ A →
-    Γ ⊢ e' ∈ A →
-    Γ ⊢ K e e' ∈ A
 
-| types_cast K p q e0 e1 :
+| types_cast K e0 e1 A B :
     Γ ⊢ e0 ∈ K →
-    Γ ⊢ e0 ; p ≡ q →
-    Γ ⊢ e1 ∈ p →
-    Γ ⊢ cast e0 e1 ∈ q
-where "Γ ⊢ x ∈ A" := (types Γ x A)
-with
-  coerces (Γ: string → term): term → term → term → Type :=
-  (* FIXME alpha conversion ? *)
-  (* also seems sus *)
-| coerces_var x: Γ ⊢ var x ; var x ≡ var x
+    e0 ; A ≡ B →
+    Γ ⊢ e1 ∈ A →
+    Γ ⊢ e1 ∈ B
+where "Γ ⊢ x ∈ A" := (types Γ x A).
 
-| coerces_set: Γ ⊢ set ; set ≡ set
-| coerces_lam x A e p p' q q':
-    Γ ⊢ A ; p ≡ p' →
-    put x A Γ ⊢ e ; q ≡ q' →
-    Γ ⊢ lam x A e ; lam x p q ≡ lam x p' q'
-| coerces_app e0 e1 p p' q q':
-    Γ ⊢ e0 ; p ≡ p' →
-    Γ ⊢ e1 ; q ≡ q' →
-    Γ ⊢ app e0 e1 ; app p q ≡ app p' q'
+Function
+  st (e: term): option (term * term) :=
+  match e with
+  | all y A e =>
+    if st A is Some (sA, tA)
+    then
+      if st e is Some (se, te)
+      then
+        Some (all y sA se, all y tA te)
+      else
+        None
+    else
+      None
 
-| coerces_cast p q r s e0 e1 :
-    Γ ⊢ e0 ; p ≡ q →
-    Γ ⊢ e1 ; r ≡ s →
-    Γ ⊢ cast e0 e1 ; r ≡ s
+  | lam y A e =>
+    if st A is Some (sA, tA)
+    then
+      if st e is Some (se, te)
+      then
+        Some (lam y sA se, lam y tA te)
+      else
+        None
+    else
+      None
 
-| coerces_trans e0 e1 p q r:
-    Γ ⊢ e0 ; p ≡ q →
-    Γ ⊢ e1 ; q ≡ r →
-    Γ ⊢ trans e0 e1 ; p ≡ r
-| coerces_sym e p q:
-    Γ ⊢ e ; p ≡ q →
-    Γ ⊢ sym e ; q ≡ p
-(* IDK here at all, weird *)
-| coerces_K e e' p q:
-    Γ ⊢ e ; p ≡ q →
-    Γ ⊢ e' ; p ≡ q →
-    Γ ⊢ K e e' ; e ≡ e'
-| coerces_beta x A e0 e1:
-    Γ ⊢ beta x A e0 e1 ; app (lam x A e0) e1 ≡ subst x e1 e0
-where "Γ ⊢ x ; P ≡ Q" := (coerces Γ x P Q).
+  | app e0 e1 =>
+    if st e0 is Some (se0, te0)
+    then
+      if st e1 is Some (se1, te1)
+      then
+        Some (app se0 se1, app te0 te1)
+      else
+        None
+    else
+      None
+
+  | e0 ∘ e1 =>
+    if st e0 is Some (se0, te0)
+    then
+      if st e1 is Some (se1, te1)
+      then
+        if term_dec se0 te1
+        then
+          Some (se1, te0)
+        else
+          None
+      else
+        None
+    else
+      None
+
+  | sym e =>
+    if st e is Some (se, te)
+    then
+      Some (te, se)
+    else
+      None
+
+  | beta y A f e => Some (app (lam y A f) e, [y := e] f)
+
+  | _ => Some (e, e)
+  end.
+
+Definition st_complete:
+  ∀ {e A B},
+  Some (A, B) = st e →
+  e ; A ≡ B.
+Proof.
+  intros e.
+  functional induction (st e).
+  all: intros ? ? p.
+  all: cbn in *.
+  all: inversion p.
+  all: subst.
+  all: try econstructor.
+  all: try eauto.
+  - apply subst_sound.
+    reflexivity.
+  - destruct e.
+    all: try contradiction.
+    all: econstructor.
+Defined.
+
+Definition st_sound:
+  ∀ {e A B},
+  e ; A ≡ B →
+  Some (A, B) = st e.
+Proof.
+  intros e.
+  induction e.
+  all: intros ? ? p.
+  all: cbn in *.
+  all: inversion p.
+  all: subst.
+  all: try reflexivity.
+  - rewrite <- (IHe1 _ _ H4).
+    rewrite <- (IHe2 _ _ H5).
+    reflexivity.
+  - rewrite <- (IHe1 _ _ H4).
+    rewrite <- (IHe2 _ _ H5).
+    reflexivity.
+  - rewrite <- (IHe1 _ _ H1).
+    rewrite <- (IHe2 _ _ H4).
+    reflexivity.
+  - rewrite <- (IHe1 _ _ H1).
+    rewrite <- (IHe2 _ _ H4).
+    destruct (term_dec q q).
+    2: contradiction.
+    reflexivity.
+  - rewrite <- (IHe _ _ H0).
+    reflexivity.
+  - rewrite (subst_complete H5).
+    reflexivity.
+Defined.
+
+Inductive normal: term → Type :=
+| norm_ofU u: normal (ofU u)
+| norm_all x A e:
+    normal A → normal e → normal (all x A e)
+| norm_var x:
+    normal (var x)
+| norm_lam x A e:
+    normal A → normal e →
+    normal (lam x A e)
+| norm_app e0 e1:
+    (∀ x A e, e0 ≠ lam x A e) →
+    normal e0 → normal e1 →
+    normal (app e0 e1)
+.
+
+Inductive nn: term → Type :=
+| nn_beta x A e0 e1:
+    nn (app (lam x A e0) e1)
+
+| nn_all x A e0:
+    nn A + nn e0 →
+    nn (all x A e0)
+| nn_lam x A e0:
+    nn A + nn e0 →
+    nn (lam x A e0)
+| nn_app e0 e1:
+    nn e0 + nn e1 →
+    nn (app e0 e1)
+.
+
+Reserved Notation "A ~> B" (at level 80).
+Inductive
+  step: term → term → Type :=
+| step_beta {x A e0 e1 e0'}:
+    substs x e0 e1 e0' →
+    app (lam x A e0) e1 ~> e0'
+
+| step_all_l {x A A' e0}:
+    A ~> A' →
+    all x A e0 ~> all x A' e0
+| step_all_r {x A e0 e0'}:
+    e0 ~> e0' →
+    all x A e0 ~> all x A e0'
+
+| step_lam_l {x A A' e0}:
+    A ~> A' →
+    lam x A e0 ~> lam x A' e0
+| step_lam_r {x A e0 e0'}:
+    e0 ~> e0' →
+    lam x A e0 ~> lam x A e0'
+
+| step_app_l {e0 e1 e0'}:
+    e0 ~> e0' →
+    app e0 e1 ~> app e0' e1
+| step_app_r {e0 e1 e1'}:
+    e1 ~> e1' →
+    app e0 e1 ~> app e0 e1'
+where "A ~> B" := (step A B).
+
+Reserved Notation "A ~>* B" (at level 80).
+Inductive
+  big: term → term → Type :=
+| halt {A}: A ~>* A
+| next {A B C}: A ~> B → B ~>* C → A ~>* C
+where "A ~>* B" := (big A B).
+
+Definition preserve_equiv:
+  ∀ {e e'},
+    e ~> e' →
+    ∀ {A B},
+    e ; A ≡ B → e' ; A ≡ B.
+Proof.
+  intros e.
+  induction e.
+  all: intros e' p.
+  all: inversion p.
+  all: subst.
+  all: intros ? ? q.
+  all: inversion q.
+  all: subst.
+  all: try econstructor.
+  all: try eauto.
+  inversion H1.
+  subst.
+Admitted.
+
+Definition preservation:
+  ∀ {e e'},
+    e ~> e' →
+    ∀ {Γ A},
+    Γ ⊢ e ∈ A → Γ ⊢ e' ∈ A.
+Proof.
+  intros e.
+  induction e.
+  all: intros e' p.
+  all: inversion p.
+  all: subst.
+  all: intros Γ T q.
+  all: inversion q.
+  all: subst.
+Admitted.
+
+Definition progress:
+  ∀ {e},
+    nn e →
+    ∀ Γ A, Γ ⊢ e ∈ A →
+    Σ e', e ~> e'.
+Proof.
+  intros e.
+  all: induction e.
+  all: intros p.
+  all: inversion p.
+  all: subst.
+  all: intros Γ T q.
+  all: inversion q.
+  all: subst.
+  - destruct H0.
+    + destruct (IHe1 n Γ _ H4) as [e1' r].
+      exists (all x e1' e2).
+      econstructor.
+      auto.
+    + destruct (IHe2 n _ _ H5) as [e2' r].
+      exists (all x e1 e2').
+      econstructor.
+      auto.
+Admitted.
+
+
+Example id := lam "A" set (lam "x" (var "A") (var "x")).
+
+Function eval e :=
+  match e with
+  | app (lam x A e0) e1 => Some (subst x e0 e1)
+
+  | app e0 e1 =>
+    if eval e0 is Some e0'
+    then
+      Some (app e0' e1)
+    else
+      if eval e1 is Some e1'
+      then
+        Some (app e0 e1')
+      else
+        None
+
+  | all x A e =>
+    if eval A is Some A'
+    then
+      Some (all x A' e)
+    else
+      if eval e is Some e'
+      then
+        Some (all x A e')
+      else
+        None
+
+  | lam x A e =>
+    if eval A is Some A'
+    then
+      Some (lam x A' e)
+    else
+      if eval e is Some e'
+      then
+        Some (lam x A e')
+      else
+        None
+
+  | _ => None
+  end.
+
+Definition eval_sound:
+  ∀ {e e'}, Some e' = eval e →
+  e ~> e'.
+Proof.
+  intros e.
+  functional induction (eval e).
+  all: intros ? p.
+  all: cbn in *.
+  all: inversion p.
+  all: subst.
+  all: cbn in *.
+  all: try econstructor.
+  all: try eauto.
+  apply subst_sound.
+  reflexivity.
+Defined.
+
+Definition eval_complete:
+  ∀ {e e'}, e ~> e' →
+  eval e = Some e'.
+Proof.
+  intros e.
+  induction e.
+  all: cbn in *.
+  all: intros e' p.
+  all: inversion p.
+  all: subst.
+  all: try (set (q := IHe1 _ H3); rewrite q).
+  all: try (set (q := IHe2 _ H3); rewrite q).
+  all: try (set (q := IHe1 _ H2); rewrite q).
+  all: try (set (q := IHe2 _ H2); rewrite q).
+  all: try reflexivity.
+Admitted.
+
+Definition tr A := ∀ (B: Prop), (A → B) → B.
+
+Program
+Fixpoint normalize {Γ A} e (p: Γ ⊢ e ∈ A) {measure e (λ x y, tr (y ~>* x))} :=
+  if eval e is Some e'
+  then
+    normalize e' (preservation (eval_sound _) p)
+  else
+    e.
+
+Next Obligation.
+Proof.
+  intros ? k.
+  apply k.
+  refine (next _ halt).
+  apply eval_sound.
+  auto.
+Defined.
+
+Next Obligation.
+Proof.
+Admitted.
